language definition

thorin/semantics/lang.v
@@ -7,291 +7,242 @@ Declare Scope val_scope.
 Delimit Scope expr_scope with E.
 Delimit Scope val_scope with V.
 
-(** Expressions and vals. *)
-Inductive base_lit : Set :=
-  | LitInt (n : Z) | LitBool (b : bool) | LitUnit.
-Inductive un_op : Set :=
-  | NegOp | MinusUnOp.
-Inductive bin_op : Set :=
-  | PlusOp | MinusOp | MultOp (* Arithmetic *)
-  | LtOp | LeOp | EqOp. (* Comparison *)
-
-
 Inductive expr :=
-  | Lit (l : base_lit)
-  (* Base lambda calculus *)
+  | Star
+  | Box
+  | Nat
+  | Idx 
+  | LitNat (n : nat)
+  | LitIdx (n : nat) (i:Fin.t n)
   | Var (x : string)
-  | Lam (x : binder) (e : expr)
+  (* let is already normalized *)
+  (* axiom is already handled *)
+  | Pi (x : binder) (T U : expr)
+  (* lam has a filter expression *)
+  | Lam (x : binder) (T : expr) (f : expr) (U: expr) (e: expr)
   | App (e1 e2 : expr)
-  (* Base types and their operations *)
-  | UnOp (op : un_op) (e : expr)
-  | BinOp (op : bin_op) (e1 e2 : expr)
-  | If (e0 e1 e2 : expr)
-  (* Polymorphism *)
-  | TApp (e : expr)
-  | TLam (e : expr)
-  | Pack (e : expr)
-  | Unpack (x : binder) (e1 e2 : expr)
-  (* Products *)
-  | Pair (e1 e2 : expr)
-  | Fst (e : expr)
-  | Snd (e : expr)
-  (* Sums *)
-  | InjL (e : expr)
-  | InjR (e : expr)
-  | Case (e0 : expr) (e1 : expr) (e2 : expr).
+  | Sigma (args: list (binder * expr))
+  | Tuple (es : list expr)
+  | Array (x: binder) (en: expr) (T: expr)
+  | Pack (x: binder) (en: expr) (e: expr)
+  | Extract (e: expr) (ei: expr)
+.
 
 Bind Scope expr_scope with expr.
 
-Inductive val :=
-  | LitV (l : base_lit)
-  | LamV (x : binder) (e : expr)
-  | TLamV (e : expr)
-  | PackV (v : val)
-  | PairV (v1 v2 : val)
-  | InjLV (v : val)
-  | InjRV (v : val)
-.
+(*
+  We argue at some points over lists.
+  We could use ∀x∈xs. P x
+  However, we want a stronger statement:
+  - Computational (not Prop)
+  - List structure linked to xs
+  - Able to use induction/destructuring on the strucutre
 
-Bind Scope val_scope with val.
+  https://ps.uni-saarland.de/~ullrich/bachelor.php
+  https://github.com/NeuralCoder3/parametricity-note
 
-Fixpoint of_val (v : val) : expr :=
-  match v with
-  | LitV l => Lit l
-  | LamV x e => Lam x e
-  | TLamV e => TLam e
-  | PackV v => Pack (of_val v)
-  | PairV v1 v2 => Pair (of_val v1) (of_val v2)
-  | InjLV v => InjL (of_val v)
-  | InjRV v => InjR (of_val v)
-  end.
-
-Fixpoint to_val (e : expr) : option val :=
-  match e with
-  | Lit l => Some $ LitV l
-  | Lam x e => Some (LamV x e)
-  | TLam e => Some (TLamV e)
-  | Pack e =>
-     to_val e ≫= (λ v, Some $ PackV v)
-  | Pair e1 e2 =>
-    to_val e1 ≫= (λ v1, to_val e2 ≫= (λ v2, Some $ PairV v1 v2))
-  | InjL e => to_val e ≫= (λ v, Some $ InjLV v)
-  | InjR e => to_val e ≫= (λ v, Some $ InjRV v)
-  | _ => None
-  end.
-
-(** Equality and other typeclass stuff *)
-Lemma to_of_val v : to_val (of_val v) = Some v.
-Proof.
-  by induction v; simplify_option_eq; repeat f_equal; try apply (proof_irrel _).
-Qed.
-
-Lemma of_to_val e v : to_val e = Some v → of_val v = e.
-Proof.
-  revert v; induction e; intros v ?; simplify_option_eq; auto with f_equal.
-Qed.
-
-#[export] Instance of_val_inj : Inj (=) (=) of_val.
-Proof. by intros ?? Hv; apply (inj Some); rewrite <-!to_of_val, Hv. Qed.
-
-(** structural computational version *)
-Fixpoint is_val (e : expr) : Prop :=
-  match e with
-  | Lit l => True
-  | Lam x e => True
-  | TLam e => True
-  | Pack e => is_val e
-  | Pair e1 e2 => is_val e1 ∧ is_val e2
-  | InjL e => is_val e
-  | InjR e => is_val e
-  | _ => False
-  end.
-Lemma is_val_spec e : is_val e ↔ ∃ v, to_val e = Some v.
-Proof.
-  induction e as [ | | ? e IH | e1 IH1 e2 IH2 | e IH | ? e1 IH1 e2 IH2 | e1 IH1 e2 IH2 e3 IH3 | e IH | e IH | e IH | ? e1 IH1 e2 IH2 | e1 IH1 e2 IH2 | e IH | e IH | e IH | e IH | e1 IH1 e2 IH2 e3 IH3 ];
-    simpl; (split; [ | intros (v & Heq)]); simplify_option_eq; try done; eauto.
-  - rewrite IH. intros (v & ->). eauto.
-  - apply IH. eauto.
-  - rewrite IH1, IH2. intros [(v1 & ->) (v2 & ->)]. eauto.
-  - rewrite IH1, IH2. eauto.
-  - rewrite IH. intros (v & ->). eauto.
-  - apply IH. eauto.
-  - rewrite IH. intros (v & ->); eauto.
-  - apply IH. eauto.
-Qed.
-
-Ltac simplify_val :=
-  repeat match goal with
-  | H: to_val (of_val ?v) = ?o |- _ => rewrite to_of_val in H
-  | H: is_val ?e |- _ => destruct (proj1 (is_val_spec e) H) as (? & ?); clear H
-  end.
-
-(* Misc *)
-Lemma is_val_of_val v : is_val (of_val v).
-Proof. apply is_val_spec. rewrite to_of_val. eauto. Qed.
-
-(* literals and our operators have decidable equality. *)
-Global Instance base_lit_eq_dec : EqDecision base_lit.
-Proof. solve_decision. Defined.
-Global Instance un_op_eq_dec : EqDecision un_op.
-Proof. solve_decision. Defined.
-Global Instance bin_op_eq_dec : EqDecision bin_op.
-Proof. solve_decision. Defined.
+  We use the unary ∀ parametricity relation
+  For lists, this is Forall.
+*)
 
 
-(** Substitution *)
+(* 
+  Semantics uses an additional val type with of_val, to_val and conversions between them.
+  They need it to simplify the definition of computational steps (e.g. un_op_eval/bin_op_eval). (but not significantly)
+
+  To me, a inductive predicate is_val seems to be shorter and simpler.
+  All our proofs only argue about is_val.
+*)
+
+Inductive is_val : expr → Prop :=
+  | StarV : is_val Star
+  | BoxV : is_val Box
+  | NatV : is_val Nat
+  | IdxV : is_val Idx
+  (* TODO: is (Idx n) a value? if not what does it reduce to *)
+  | IdxAppV n : is_val (App Idx (LitNat n))
+  | LitNatV n : is_val (LitNat n)
+  | LitIdxV n i : is_val (LitIdx n i)
+  | PiV x T U : is_val (Pi x T U)
+  | LamV x T f U e : 
+    is_val T →
+    (* U might depend on x:T *)
+    is_val (Lam x T f U e)
+  (* compound values *)
+  (* sigma would not be strictly positive
+    => either two lists or use the val type
+
+    however, sigma is like lambda (functions depending on previous values)
+    => only the first one should be a val
+  *)
+  | SigmaEmptyV: is_val (Sigma [])
+  (* we do not need to test the rest => (implicitely) depends on first one *)
+  | SigmaConsV x T args : is_val T → is_val (Sigma ((x, T) :: args))
+  | TupleV es : Forall is_val es → is_val (Tuple es)
+  | ArrayV x en T : 
+    is_val en →
+    is_val (Array x en T)
+  | PackV x en e :
+    is_val en →
+    is_val (Pack x en e)
+  .
+
+(* Definition subst_if_not subst (b:binder) (x:string) (es:expr) (e:expr) :=
+  if decide (b = BNamed x) then e else subst x es e. *)
+
+
 Fixpoint subst (x : string) (es : expr) (e : expr)  : expr :=
+  (* let recursive_under y expr := subst_if_not subst y x es expr in *)
+  let recurse_under y expr := if decide (y = BNamed x) then expr else subst x es expr in
   match e with
-  | Lit _ => e
-  | Var y => if decide (x = y) then es else Var y
-  | Lam y e =>
-      Lam y $ if decide (BNamed x = y) then e else subst x es e
+  | Star | Box | Nat | Idx | LitNat _ | LitIdx _ _ | Var _ => e
+  (* replace x in T, replace in U if not x *)
+  | Pi y T U => 
+    (* Pi y (subst x es T) (subst_if_not subst y x es U) *)
+    Pi y (subst x es T) (recurse_under y U)
+  (* replace x in T, f, U, and e only if not x *)
+  | Lam y T f U e => 
+    Lam y (subst x es T) 
+      (recurse_under y f)
+      (recurse_under y U)
+      (recurse_under y e)
+      (* (subst_if_not subst y x es f) 
+      (subst_if_not subst y x es U) 
+      (subst_if_not subst y x es e) *)
   | App e1 e2 => App (subst x es e1) (subst x es e2)
-  | TApp e => TApp (subst x es e)
-  | TLam e => TLam (subst x es e)
-  | Pack e => Pack (subst x es e)
-  | Unpack y e1 e2 => Unpack y (subst x es e1) (if decide (BNamed x = y) then e2 else subst x es e2)
-  | UnOp op e => UnOp op (subst x es e)
-  | BinOp op e1 e2 => BinOp op (subst x es e1) (subst x es e2)
-  | If e0 e1 e2 => If (subst x es e0) (subst x es e1) (subst x es e2)
-  | Pair e1 e2 => Pair (subst x es e1) (subst x es e2)
-  | Fst e => Fst (subst x es e)
-  | Snd e => Snd (subst x es e)
-  | InjL e => InjL (subst x es e)
-  | InjR e => InjR (subst x es e)
-  | Case e0 e1 e2 => Case (subst x es e0) (subst x es e1) (subst x es e2)
+  (* | Sigma [] => Sigma []
+  | Sigma ((y, T) :: args) => Sigma ((y, subst x es T) :: map (λ '(y, T), (y, subst x es T)) args) *)
+  (* map over nested induction 
+  => use inner fixpoint 
+  mutual recursion is not recognized (https://coq.discourse.group/t/mutual-recursion-for-nested-inductive-types/729/3)
+  Equations would be possible but not necessarily easier
+   *)
+  | Tuple expression =>
+    Tuple (map (subst x es) expression)
+    (* Tuple ((fix map_subst (es' : list expr) : list expr :=
+      match es' with
+      | [] => []
+      | e :: es' => subst x es e :: map_subst es'
+      end) expression) *)
+  (* for Sigma, we only continue subst in args if not already encountered var *)
+  | Sigma xs =>
+    Sigma ((fix fold_subst (xs : list (binder * expr)) : list (binder * expr) :=
+      match xs with
+      | [] => []
+      | (y, T) :: xs => 
+        (* stop at [x:..., ...] => later x are regarding the parameter*)
+        (y, subst x es T) :: (if decide (y = BNamed x) then xs else fold_subst xs)
+      end) xs)
+  | Array y en T => Array y (subst x es en) (recurse_under y T)
+  | Pack y en e => Pack y (subst x es en) (recurse_under y e)
+  | Extract e ei => Extract (subst x es e) (subst x es ei)
   end.
 
 Definition subst' (mx : binder) (es : expr) : expr → expr :=
   match mx with BNamed x => subst x es | BAnon => id end.
 
-(** The stepping relation *)
-Definition un_op_eval (op : un_op) (v : val) : option val :=
-  match op, v with
-  | NegOp, LitV (LitBool b) => Some $ LitV $ LitBool (negb b)
-  | MinusUnOp, LitV (LitInt n) => Some $ LitV $ LitInt (- n)
-  | _, _ => None
-  end.
+(* https://coq.inria.fr/doc/v8.18/refman/language/core/conversion.html *)
+Inductive base_step : expr -> expr -> Prop :=
+(* 'real' steps (congruence steps later) *)
+  | BetaS x T f U elam earg e' :
+  (* TODO: necessary to completely eval T? should probably be *)
+    is_val T ->
+    is_val earg ->
+    e' = subst' x earg elam ->
+    base_step (App (Lam x T f U elam) earg) e'
+  | IotaTupleS es n (i:Fin.t n) e:
+    (* extract from a tuple if all value *)
+    (* needs canonical form lemma for Idx n *)
+    (*
+    for nth, we need a proof about the size
+    alternatively, a vector would work but we would have the size everywhere
+    *)
+    Forall is_val es ->
+    length es = n ->
+    nth_error es (` (Fin.to_nat i)) = Some e ->
+    base_step (Extract (Tuple es) (LitIdx n i)) e
+  (* extract of pack *)
+  | IotaPackS x e n ei e':
+    (* ei = LitIdx n i -> *)
+    is_val ei -> (* implies ei = LitIdx n i *)
+    e' = subst' x ei e ->
+    base_step (Extract (Pack x (LitNat n) e) ei) e'
+  .
 
-Definition bin_op_eval_int (op : bin_op) (n1 n2 : Z) : option base_lit :=
-  match op with
-  | PlusOp => Some $ LitInt (n1 + n2)
-  | MinusOp => Some $ LitInt (n1 - n2)
-  | MultOp => Some $ LitInt (n1 * n2)
-  | LtOp => Some $ LitBool (bool_decide (n1 < n2))
-  | LeOp => Some $ LitBool (bool_decide (n1 ≤ n2))
-  | EqOp => Some $ LitBool (bool_decide (n1 = n2))
-  end%Z.
 
-Definition bin_op_eval (op : bin_op) (v1 v2 : val) : option val :=
-  match v1, v2 with
-  | LitV (LitInt n1), LitV (LitInt n2) => LitV <$> bin_op_eval_int op n1 n2
-  | _, _ => None
-  end.
+Lemma fin_inc n (i:Fin.t n): (` (Fin.to_nat (Fin.FS i))) = S (` (Fin.to_nat i)).
+Proof.
+  induction i; simpl.
+  - reflexivity.
+  - admit.
+Admitted.
 
-Inductive base_step : expr → expr → Prop :=
-  | BetaS x e1 e2 e' :
-     is_val e2 →
-     e' = subst' x e2 e1 →
-     base_step (App (Lam x e1) e2) e'
-  | TBetaS e1 :
-      base_step (TApp (TLam e1)) e1
-  | UnpackS e1 e2 e' x :
-      is_val e1 →
-      e' = subst' x e1 e2 →
-      base_step (Unpack x (Pack e1) e2) e'
-  | UnOpS op e v v' :
-     to_val e = Some v →
-     un_op_eval op v = Some v' →
-     base_step (UnOp op e) (of_val v')
-  | BinOpS op e1 v1 e2 v2 v' :
-     to_val e1 = Some v1 →
-     to_val e2 = Some v2 →
-     bin_op_eval op v1 v2 = Some v' →
-     base_step (BinOp op e1 e2) (of_val v')
-  | IfTrueS e1 e2 :
-     base_step (If (Lit $ LitBool true) e1 e2) e1
-  | IfFalseS e1 e2 :
-     base_step (If (Lit $ LitBool false) e1 e2) e2
-  | FstS e1 e2 :
-     is_val e1 →
-     is_val e2 →
-     base_step (Fst (Pair e1 e2)) e1
-  | SndS e1 e2 :
-     is_val e1 →
-     is_val e2 →
-     base_step (Snd (Pair e1 e2)) e2
-  | CaseLS e e1 e2 :
-     is_val e →
-     base_step (Case (InjL e) e1 e2) (App e1 e)
-  | CaseRS e e1 e2 :
-     is_val e →
-     base_step (Case (InjR e) e1 e2) (App e2 e)
-.
+Lemma nth_fin A (xs:list A) (i:Fin.t (length xs)) :
+  exists x, nth_error xs (` (Fin.to_nat i)) = Some x.
+Proof.
+  induction xs;simpl in *.
+  - inversion i.
+  - dependent inversion i;subst.
+    + now exists a.
+    + specialize (IHxs t) as [x H].
+      exists x.
+      rewrite <- H.
+      now rewrite fin_inc.
+Qed.
 
-(** We define evaluation contexts *)
+(* evaluation contexts for congruence reduction *)
+(* a hole/context is an evaluation point *)
+(* TODO: do we want to restrict context to only have hole right if value left? *)
 Inductive ectx :=
   | HoleCtx
-  | AppLCtx (K: ectx) (v2 : val)
+  (* only context in T as U might depend on x:T *)
+  | PiCtx (x:binder) (K: ectx) (U:expr)
+  | LamCtx (x:binder) (K: ectx) (f:expr) (U:expr) (e:expr)
+  | AppLCtx (K: ectx) (v2 : expr)
   | AppRCtx (e1 : expr) (K: ectx)
-  | TAppCtx (K: ectx)
-  | PackCtx (K: ectx)
-  | UnpackCtx (x : binder)(K: ectx)  (e2 : expr)
-  | UnOpCtx (op : un_op) (K: ectx)
-  | BinOpLCtx (op : bin_op) (K: ectx) (v2 : val)
-  | BinOpRCtx (op : bin_op) (e1 : expr) (K: ectx)
-  | IfCtx (K: ectx) (e1 e2 : expr)
-  | PairLCtx (K: ectx) (v2 : val)
-  | PairRCtx (e1 : expr) (K: ectx)
-  | FstCtx (K: ectx)
-  | SndCtx (K: ectx)
-  | InjLCtx (K: ectx)
-  | InjRCtx (K: ectx)
-  | CaseCtx (K: ectx) (e1 : expr) (e2 : expr) .
+  (* only first argument in sigma *)
+  | SigmaCtx (x:binder) (K: ectx) (args: list (binder * expr))
+  | TupleCtx (es1:list expr) (K: ectx) (es2: list expr)
+  (* only en is up to be a context *)
+  | ArrayCtx (x:binder) (K: ectx) (T:expr)
+  | PackCtx (x:binder) (K: ectx) (e:expr)
+  | ExtractLCtx (K: ectx) (ei:expr)
+  | ExtractRCtx (e:expr) (K: ectx)
+  .  
 
+(* Place an expression into the hole of a context *)
 Fixpoint fill (K : ectx) (e : expr) : expr :=
   match K with
   | HoleCtx => e
-  | AppLCtx K v2 => App (fill K e) (of_val v2)
+  | PiCtx x K U => Pi x (fill K e) U
+  | LamCtx x K f U e => Lam x (fill K e) f U e
+  | AppLCtx K v2 => App (fill K e) v2
   | AppRCtx e1 K => App e1 (fill K e)
-  | TAppCtx K => TApp (fill K e)
-  | PackCtx K => Pack (fill K e)
-  | UnpackCtx x K e2 => Unpack x (fill K e) e2
-  | UnOpCtx op K => UnOp op (fill K e)
-  | BinOpLCtx op K v2 => BinOp op (fill K e) (of_val v2)
-  | BinOpRCtx op e1 K => BinOp op e1 (fill K e)
-  | IfCtx K e1 e2 => If (fill K e) e1 e2
-  | PairLCtx K v2 => Pair (fill K e) (of_val v2)
-  | PairRCtx e1 K => Pair e1 (fill K e)
-  | FstCtx K => Fst (fill K e)
-  | SndCtx K => Snd (fill K e)
-  | InjLCtx K => InjL (fill K e)
-  | InjRCtx K => InjR (fill K e)
-  | CaseCtx K e1 e2 => Case (fill K e) e1 e2
+  | SigmaCtx x K args => Sigma ((x, fill K e) :: args)
+  | TupleCtx es1 K es2 => Tuple (es1 ++ fill K e :: es2)
+  | ArrayCtx x K T => Array x (fill K e) T
+  | PackCtx x K e => Pack x (fill K e) e
+  | ExtractLCtx K ei => Extract (fill K e) ei
+  | ExtractRCtx e K => Extract e (fill K e)
   end.
 
-Fixpoint comp_ectx (K: ectx) (K' : ectx) : ectx :=
-  match K with
-  | HoleCtx => K'
-  | AppLCtx K v2 => AppLCtx (comp_ectx K K') v2
-  | AppRCtx e1 K => AppRCtx e1 (comp_ectx K K')
-  | TAppCtx K => TAppCtx (comp_ectx K K')
-  | PackCtx K => PackCtx (comp_ectx K K')
-  | UnpackCtx x K e2 => UnpackCtx x (comp_ectx K K') e2
-  | UnOpCtx op K => UnOpCtx op (comp_ectx K K')
-  | BinOpLCtx op K v2 => BinOpLCtx op (comp_ectx K K') v2
-  | BinOpRCtx op e1 K => BinOpRCtx op e1 (comp_ectx K K')
-  | IfCtx K e1 e2 => IfCtx (comp_ectx K K') e1 e2
-  | PairLCtx K v2 => PairLCtx (comp_ectx K K') v2
-  | PairRCtx e1 K => PairRCtx e1 (comp_ectx K K')
-  | FstCtx K => FstCtx (comp_ectx K K')
-  | SndCtx K => SndCtx (comp_ectx K K')
-  | InjLCtx K => InjLCtx (comp_ectx K K')
-  | InjRCtx K => InjRCtx (comp_ectx K K')
-  | CaseCtx K e1 e2 => CaseCtx (comp_ectx K K') e1 e2
+(* Compose two evaluation contexts => place the second context into the hole of the first *)
+Fixpoint comp_ectx (K1: ectx) (K2 : ectx) : ectx :=
+  match K1 with
+  | HoleCtx => K2
+  | PiCtx x K U => PiCtx x (comp_ectx K K2) U
+  | LamCtx x K f U e => LamCtx x (comp_ectx K K2) f U e
+  | AppLCtx K v2 => AppLCtx (comp_ectx K K2) v2
+  | AppRCtx e1 K => AppRCtx e1 (comp_ectx K K2)
+  | SigmaCtx x K args => SigmaCtx x (comp_ectx K K2) args
+  | TupleCtx es1 K es2 => TupleCtx es1 (comp_ectx K K2) es2
+  | ArrayCtx x K T => ArrayCtx x (comp_ectx K K2) T
+  | PackCtx x K e => PackCtx x (comp_ectx K K2) e
+  | ExtractLCtx K ei => ExtractLCtx (comp_ectx K K2) ei
+  | ExtractRCtx e K => ExtractRCtx e (comp_ectx K K2)
   end.
 
-(** Contextual steps *)
+(** Contextual steps => lift reductions via contexts *)
 Inductive contextual_step (e1 : expr) (e2 : expr) : Prop :=
   Ectx_step K e1' e2' :
     e1 = fill K e1' → e2 = fill K e2' →
@@ -307,10 +258,27 @@ Definition empty_ectx := HoleCtx.
 Lemma fill_empty e : fill empty_ectx e = e.
 Proof. done. Qed.
 
+
+
+
+
+
+
+
+
+
+
+
+
+
+
+
+
+
+
+
 Lemma fill_comp (K1 K2 : ectx) e : fill K1 (fill K2 e) = fill (comp_ectx K1 K2) e.
 Proof. induction K1; simpl; congruence. Qed.
-
-
 
 Lemma base_contextual_step e1 e2 :
   base_step e1 e2 → contextual_step e1 e2.
@@ -455,62 +423,62 @@ Lemma contextual_step_pair_l e1 e1' e2:
   contextual_step e1 e1' →
   contextual_step (Pair e1 e2) (Pair e1' e2).
 Proof.
-  intros [v <-%of_to_val]%is_val_spec Hcontextual.
-  by eapply (fill_contextual_step (PairLCtx HoleCtx v)).
+intros [v <-%of_to_val]%is_val_spec Hcontextual.
+by eapply (fill_contextual_step (PairLCtx HoleCtx v)).
 Qed.
 
 Lemma contextual_step_pair_r e1 e2 e2':
-  contextual_step e2 e2' →
-  contextual_step (Pair e1 e2) (Pair e1 e2').
+contextual_step e2 e2' →
+contextual_step (Pair e1 e2) (Pair e1 e2').
 Proof.
-  intros Hcontextual.
-  by eapply (fill_contextual_step (PairRCtx e1 HoleCtx)).
+intros Hcontextual.
+by eapply (fill_contextual_step (PairRCtx e1 HoleCtx)).
 Qed.
 
 
 Lemma contextual_step_fst e e':
-  contextual_step e e' →
-  contextual_step (Fst e) (Fst e').
+contextual_step e e' →
+contextual_step (Fst e) (Fst e').
 Proof.
-  intros Hcontextual.
-  by eapply (fill_contextual_step (FstCtx HoleCtx)).
+intros Hcontextual.
+by eapply (fill_contextual_step (FstCtx HoleCtx)).
 Qed.
 
 Lemma contextual_step_snd e e':
-  contextual_step e e' →
-  contextual_step (Snd e) (Snd e').
+contextual_step e e' →
+contextual_step (Snd e) (Snd e').
 Proof.
-  intros Hcontextual.
-  by eapply (fill_contextual_step (SndCtx HoleCtx)).
+intros Hcontextual.
+by eapply (fill_contextual_step (SndCtx HoleCtx)).
 Qed.
 
 Lemma contextual_step_injl e e':
-  contextual_step e e' →
-  contextual_step (InjL e) (InjL e').
-  Proof.
-    intros Hcontextual.
-    by eapply (fill_contextual_step (InjLCtx HoleCtx)).
-  Qed.
-
-Lemma contextual_step_injr e e':
-  contextual_step e e' →
-  contextual_step (InjR e) (InjR e').
-  Proof.
-    intros Hcontextual.
-    by eapply (fill_contextual_step (InjRCtx HoleCtx)).
-  Qed.
-
-Lemma contextual_step_case e e' e1 e2:
-  contextual_step e e' →
-  contextual_step (Case e e1 e2) (Case e' e1 e2).
+contextual_step e e' →
+contextual_step (InjL e) (InjL e').
 Proof.
   intros Hcontextual.
-  by eapply (fill_contextual_step (CaseCtx HoleCtx e1 e2)).
+  by eapply (fill_contextual_step (InjLCtx HoleCtx)).
+Qed.
+
+Lemma contextual_step_injr e e':
+contextual_step e e' →
+contextual_step (InjR e) (InjR e').
+Proof.
+  intros Hcontextual.
+  by eapply (fill_contextual_step (InjRCtx HoleCtx)).
+Qed.
+
+Lemma contextual_step_case e e' e1 e2:
+contextual_step e e' →
+contextual_step (Case e e1 e2) (Case e' e1 e2).
+Proof.
+intros Hcontextual.
+by eapply (fill_contextual_step (CaseCtx HoleCtx e1 e2)).
 Qed.
 
 #[export]
 Hint Resolve
-  contextual_step_app_l contextual_step_app_r contextual_step_binop_l contextual_step_binop_r
-  contextual_step_case contextual_step_fst contextual_step_if contextual_step_injl contextual_step_injr
-  contextual_step_pack contextual_step_pair_l contextual_step_pair_r contextual_step_snd contextual_step_tapp
-  contextual_step_tapp contextual_step_unop contextual_step_unpack : core.
+contextual_step_app_l contextual_step_app_r contextual_step_binop_l contextual_step_binop_r
+contextual_step_case contextual_step_fst contextual_step_if contextual_step_injl contextual_step_injr
+contextual_step_pack contextual_step_pair_l contextual_step_pair_r contextual_step_snd contextual_step_tapp
+contextual_step_tapp contextual_step_unop contextual_step_unpack : core.
